

Supplementary Material on Solving SVM Duality

Wan-Lei Zhao

December 17, 2024

1 Solve the dual problem of SVM model

Overall, W is a vector, it is a sum of m vectors:

$$W = \sum_{i=1}^m \alpha_i y^{(i)} x^{(i)} \quad (5)$$

Expand Eqn. 5, we have

$$W = \alpha_1 y^{(1)} x^{(1)} + \alpha_2 y^{(2)} x^{(2)} + \dots + \alpha_i y^{(i)} x^{(i)} + \dots + \alpha_m y^{(m)} x^{(m)}$$

So

$$\begin{aligned} \|W\|^2 &= W^T \cdot W \\ &= (\alpha_1 y^{(1)} \cdot x^{(1)T} + \alpha_2 y^{(2)} \cdot x^{(2)T} + \dots + \alpha_i y^{(i)} \cdot x^{(i)T} + \dots + \alpha_m y^{(m)} \cdot x^{(m)T}) \\ &\quad \cdot (\alpha_1 y^{(1)} \cdot x^{(1)} + \alpha_2 y^{(2)} \cdot x^{(2)} + \dots + \alpha_j y^{(j)} \cdot x^{(j)} + \dots + \alpha_m y^{(m)} \cdot x^{(m)}) \\ &= \alpha_1 y^{(1)} \cdot x^{(1)T} \cdot (\alpha_1 y^{(1)} \cdot x^{(1)} + \alpha_2 y^{(2)} \cdot x^{(2)} + \dots + \alpha_j y^{(j)} \cdot x^{(j)} + \dots + \alpha_m y^{(m)} \cdot x^{(m)}) \\ &\quad + \alpha_2 y^{(2)} \cdot x^{(2)T} \cdot (\alpha_1 y^{(1)} \cdot x^{(1)} + \alpha_2 y^{(2)} \cdot x^{(2)} + \dots + \alpha_j y^{(j)} \cdot x^{(j)} + \dots + \alpha_m y^{(m)} \cdot x^{(m)}) \\ &\quad \dots \\ &\quad + \\ &\quad \dots \\ &\quad + \alpha_m y^{(m)} \cdot x^{(m)T} \cdot (\alpha_1 y^{(1)} \cdot x^{(1)} + \alpha_2 y^{(2)} \cdot x^{(2)} + \dots + \alpha_j y^{(j)} \cdot x^{(j)} + \dots + \alpha_m y^{(m)} \cdot x^{(m)}) \\ &= \sum_{i,j=1}^m y^i y^j \cdot \alpha_i \alpha_j \cdot x^{(i)T} \cdot x^{(j)} \\ &= \sum_{i,j=1}^m y^i y^j \cdot \alpha_i \alpha_j < x^{(i)}, x^{(j)} > \end{aligned}$$

For

$$\begin{aligned} &- \left[\sum_{i=1}^m \alpha_i y^{(i)} (W^T \cdot x^{(i)} + b) - \sum_{i=1}^m \alpha_i \right] \\ \Rightarrow &- \sum_{i=1}^m \alpha_i y^{(i)} W^T \cdot x^{(i)} - \sum_{i=1}^m \alpha_i y^{(i)} \cdot b + \sum_{i=1}^m \alpha_i \quad \left(\text{according to Eqn. 6, } \sum_{i=1}^m \alpha_i y^{(i)} \cdot b = 0 \right) \\ \Rightarrow &- \sum_{i=1}^m \alpha_i y^{(i)} \cdot (\alpha_1 y^{(1)} \cdot x^{(1)T} + \alpha_2 y^{(2)} \cdot x^{(2)T} + \dots + \alpha_j y^{(j)} \cdot x^{(j)T} + \dots) \cdot x^{(i)} \\ \Rightarrow &- \sum_{i,j=1}^m \alpha_i \alpha_j y^{(i)} y^{(j)} x^{(j)T} \cdot x^{(i)} + \sum_{i=1}^m \alpha_i \end{aligned}$$

Summarize above:

$$\begin{aligned} &\frac{1}{2} \|W\|^2 - \left[\sum_{i=1}^m \alpha_i y^{(i)} (W^T \cdot x^{(i)} + b) - \sum_{i=1}^m \alpha_i \right] \\ &= -\frac{1}{2} \sum_{i,j=1}^m \alpha_i \alpha_j y^{(i)} y^{(j)} x^{(i)T} \cdot x^{(j)} + \sum_{i=1}^m \alpha_i \\ &= -\frac{1}{2} \sum_{i,j=1}^m \alpha_i \alpha_j y^{(i)} y^{(j)} < x^{(i)}, x^{(j)} > + \sum_{i=1}^m \alpha_i \end{aligned}$$